ironfleet/ravana/RefinementProof/ControllerRecvEvent.dfy
@@ -39,6 +39,7 @@ module Refinement_Proof_ControllerRecvEvent {
     lemma_packets_are_valid(rs, rs');
 
     lemma_recved_events_valid(rs, rs');
+    lemma_controllers_log_valid_if_log_copy_unchanged(rs, rs');
 
     assert refinement_switchStates(rs.server_switches)
         == refinement_switchStates(rs'.server_switches);
